src/dafny/Capability.dfy
@@ -1,19 +1,19 @@
 
 
 class Capability {
-    var subspace: (int,int)
+    var subspace: set<int>
     var stack: seq<int>
     var files: seq<int>
     var entries: seq<string>
 
     constructor () {
-        subspace := (0,0);
+        subspace := {};
         stack := [];
         files := [];
         entries := [];
     }
 
-    constructor setCapability (subspace:(int,int), files:seq<int>) {
+    constructor setCapability (subspace:set<int>, files:seq<int>) {
         this.subspace := subspace;
         this.files := files;
     }
