src/dafny/Instructions.dfy
@@ -1,11 +1,4 @@
 datatype Instruction = 
     Write(fd:int, addr:int, size:int) 
-    | Read(addr:int)
+    | Read(fd:int, addr:int, size:int) 
 
-
-
-function method isWriteInstruction(i:Instruction) : bool {
-    match i 
-        case Write(fd, addr, size) => true
-        case Read(addr) => false
-}
